refractor : changed imports and added finished LJFPS rules

src/rules/LJF4_Rules.v
@@ -1,134 +1,134 @@
 From Stdlib Require Import List.
 
-From CARVe Require Import contexts.list algebras.dill.
+From CARVe Require Import contexts.list.
+From CARVe Require Import algebras.dill.
 
-Global Arguments upd_rel_ex  {R A} _ _ _ _.
 
 From LJF Require Import SharedLogic. 
 
-Inductive bct : ctx -> o -> Prop :=
-| bct_R_box :
-  forall {C: ctx} {D: o},
+Inductive bctLJF4 : dctx -> o -> Prop :=
+| bctLJF4_R_box :
+  forall {C: dctx} {D: o},
     bracketable D ->
-    ept C D ->
-    bct C D
-| bct_R_AndN :
-  forall {C: ctx} {B1 B2: o},
-    bct C B1 ->
-    bct C B2 ->
-    bct C (AndN B1 B2)
-| bct_R_Impl :
-  forall {C : ctx} {B1 B2: o},
-    bct ((B1, one) :: C) B2 ->
-    bct C (Impl B1 B2)
-
-with ept : ctx -> o -> Prop :=
-| ept_L_f :
-  forall {C: ctx} {N : o} {K : o},
+    eptLJF4 C D ->
+    bctLJF4 C D
+| bctLJF4_R_AndN :
+  forall {C: dctx} {B1 B2: o},
+    bctLJF4 C B1 ->
+    bctLJF4 C B2 ->
+    bctLJF4 C (AndN B1 B2)
+| bctLJF4_R_Impl :
+  forall {C : dctx} {B1 B2: o},
+    bctLJF4 ((B1, one) :: C) B2 ->
+    bctLJF4 C (Impl B1 B2)
+with eptLJF4 : dctx -> o -> Prop :=
+| eptLJF4_L_f :
+  forall {C: dctx} {N : o} {K : o},
     exh C ->
     has_entry C (N, omega) ->
     negative N ->
-    lfc C N K ->
-    ept C K
-| ept_R_f :
-  forall {C: ctx} {P: o},
+    lfcLJF4 C N K ->
+    eptLJF4 C K
+| eptLJF4_R_f :
+  forall {C: dctx} {P: o},
     exh C ->
     positive P ->
-    rfc C P ->
-    ept C P
-| ept_L_box :
-  forall {C C1 : ctx} {B : o} {K : o},
+    rfcLJF4 C P ->
+    eptLJF4 C P
+| eptLJF4_L_box :
+  forall {C C1 : dctx} {B : o} {K : o},
+    has_entry C (B, one) ->
     upd_rel_ex C (B, one) (B, omega) C1 ->
     permeable B ->
-    ept C1 K ->
-    ept C K
-| ept_L_AndP :
-  forall {C C1: ctx} {B1 B2 : o} {K: o},
+    eptLJF4 C1 K ->
+    eptLJF4 C K
+| eptLJF4_L_AndP :
+  forall {C C1: dctx} {B1 B2 : o} {K: o},
     has_entry C ((AndP B1 B2), one) ->
     upd_rel_ex C ((AndP B1 B2), one) ((AndP B1 B2), zero) C1 ->
-    ept ((B1, one) :: (B2, one) :: C1) K ->
-    ept C K
-| ept_L_Or :
-  forall {C C1: ctx} {B1 B2 : o}  {K: o},
+    eptLJF4 ((B1, one) :: (B2, one) :: C1) K ->
+    eptLJF4 C K
+| eptLJF4_L_Or :
+  forall {C C1: dctx} {B1 B2 : o}  {K: o},
     has_entry C ((Or B1 B2), one) ->
     upd_rel_ex C ((Or B1 B2), one) ((Or B1 B2), zero) C1 ->
-    ept ((B1, one) :: C1) K ->
-    ept ((B2, one) :: C1) K ->
-    ept C K
-| ept_L_True :
-  forall {C C1: ctx}  {K: o},
+    eptLJF4 ((B1, one) :: C1) K ->
+    eptLJF4 ((B2, one) :: C1) K ->
+    eptLJF4 C K
+| eptLJF4_L_True :
+  forall {C C1: dctx}  {K: o},
     has_entry C (TT, one) ->
     upd_rel_ex C (TT, one) (TT, zero) C1 ->
-    ept C1 K ->
-    ept C K
-| ept_L_False :
-  forall {C: ctx}  {K: o},
+    eptLJF4 C1 K ->
+    eptLJF4 C K
+| eptLJF4_L_False :
+  forall {C: dctx}  {K: o},
     has_entry C (FF, one) ->
-    ept C K
+    eptLJF4 C K
 
 (* First o for focused assumption, second o for conclusion K *)
-with lfc : ctx -> o -> o -> Prop :=
-| lfc_R_l :
-  forall {C : ctx} {P : o}  {K : o},
+with lfcLJF4 : dctx -> o -> o -> Prop :=
+| lfcLJF4_R_l :
+  forall {C : dctx} {P : o}  {K : o},
     exh C ->
     positive P ->
-    ept ((P, one) :: C) K ->
-    lfc C P K
-| lfc_I_l :
-  forall {C: ctx} {N : o},
+    eptLJF4 ((P, one) :: C) K ->
+    lfcLJF4 C P K
+| lfcLJF4_I_l :
+  forall {C: dctx} {N : o},
     exh C ->
     negative N ->
     atomic N ->
-    lfc C N N
-| lfc_L_AndN_1 :
-  forall {C: ctx} {B1 B2 : o}  {K : o},
+    lfcLJF4 C N N
+| lfcLJF4_L_AndN_1 :
+  forall {C: dctx} {B1 B2 : o}  {K : o},
     exh C ->
-    lfc C B1 K ->
-    lfc C (AndN B1 B2) K
-| lfc_L_AndN_2 :
-  forall {C: ctx} {B1 B2 : o}  {K : o},
+    lfcLJF4 C B1 K ->
+    lfcLJF4 C (AndN B1 B2) K
+| lfcLJF4_L_AndN_2 :
+  forall {C: dctx} {B1 B2 : o}  {K : o},
     exh C ->
-    lfc C B2 K ->
-    lfc C (AndN B1 B2) K
-| lfc_L_Impl :
-  forall {C: ctx} {B1 B2 : o}  {K : o},
+    lfcLJF4 C B2 K ->
+    lfcLJF4 C (AndN B1 B2) K
+| lfcLJF4_L_Impl :
+  forall {C: dctx} {B1 B2 : o}  {K : o},
     exh C ->
-    rfc C B1 ->
-    lfc C B2 K ->
-    lfc C (Impl B1 B2) K
+    rfcLJF4 C B1 ->
+    lfcLJF4 C B2 K ->
+    lfcLJF4 C (Impl B1 B2) K
 
-with rfc : ctx -> o -> Prop :=
-| rfc_R_r :
-  forall {C: ctx} {N: o},
+with rfcLJF4 : dctx -> o -> Prop :=
+| rfcLJF4_R_r :
+  forall {C: dctx} {N: o},
     exh C ->
     negative N ->
-    bct C N ->
-    rfc C N
-| rfc_I_r :
-  forall {C: ctx} {P: o},
+    bctLJF4 C N ->
+    rfcLJF4 C N
+| rfcLJF4_I_r :
+  forall {C: dctx} {P: o},
     exh C ->
     has_entry C (P, omega) ->
     positive P ->
     atomic P ->
-    rfc C P
-| rfc_R_AndP :
-  forall {C: ctx} {B1 B2: o},
+    rfcLJF4 C P
+| rfcLJF4_R_AndP :
+  forall {C: dctx} {B1 B2: o},
     exh C ->
-    rfc C B1 ->
-    rfc C B2 ->
-    rfc C (AndP B1 B2)
-| rfc_R_Or_1 :
-  forall {C: ctx} {B1 B2: o},
+    rfcLJF4 C B1 ->
+    rfcLJF4 C B2 ->
+    rfcLJF4 C (AndP B1 B2)
+| rfcLJF4_R_Or_1 :
+  forall {C: dctx} {B1 B2: o},
     exh C ->
-    rfc C B1 ->
-    rfc C (Or B1 B2)
-| rfc_R_Or_2 :
-  forall {C: ctx} {B1 B2: o},
+    rfcLJF4 C B1 ->
+    rfcLJF4 C (Or B1 B2)
+| rfcLJF4_R_Or_2 :
+  forall {C: dctx} {B1 B2: o},
     exh C ->
-    rfc C B2 ->
-    rfc C (Or B1 B2)
-| rfc_R_True :
-  forall {C: ctx},
+    rfcLJF4 C B2 ->
+    rfcLJF4 C (Or B1 B2)
+| rfcLJF4_R_True :
+  forall {C: dctx},
     exh C ->
-    rfc C TT
+    rfcLJF4 C TT
 .
