src/examples/LJF4_Test.v
@@ -1,11 +1,9 @@
 From Stdlib Require Import List.
-
 From CARVe Require Import contexts.list algebras.dill.
-
 From LJF Require Import LJF4_Rules LJF4_Prover SharedLogic.
 
 
-Lemma True_proveable: bct nil TT.
+Lemma True_proveable: bctLJF4 nil TT.
 Proof. T_solve. Qed.
 
 
@@ -14,7 +12,7 @@ Lemma Impl_trans_backward_chaining : forall (x y z : nat),
   let b := Atom Neg y in
   let c := Atom Neg z in
   let C := (a, omega) :: (Impl a b, omega) :: (Impl b c, omega) :: nil in
-  lfc C (Impl b c) c.
+  lfcLJF4 C (Impl b c) c.
 Proof. T_solve. Qed.
 
 Lemma Impl_trans_forward_chaining : forall (x y z : nat),
@@ -22,7 +20,7 @@ Lemma Impl_trans_forward_chaining : forall (x y z : nat),
   let b := Atom Pos y in
   let c := Atom Neg z in
   let C := (a, omega) :: (Impl a b, omega) :: (Impl b c, omega) :: nil in
-  lfc C (Impl a b) c.
+  lfcLJF4 C (Impl a b) c.
 Proof. T_solve. Qed.
 
 
@@ -31,5 +29,5 @@ Lemma Impl_trans : forall (x y z : nat),
   let b := Atom Neg y in
   let c := Atom Neg z in
   let C := (a, omega) :: (Impl a b, omega) :: (Impl b c, omega) :: nil in
-  bct C c.
+  bctLJF4 C c.
 Proof. T_solve. Qed.
