src/metatheory/LJF4_Completeness.v
@@ -1,0 +1,39 @@
+From Stdlib Require Import List.
+From CARVe Require Import contexts.list.
+From CARVe Require Import algebras.dill.
+From LJF Require Import SharedLogic LJF_Rules LJF4_Rules LJF4_Prover.
+
+Lemma admissibility_L_false : forall (R : o) (C: dctx), 
+    has_entry C (FF, one) -> bctLJF4 C R.
+Proof. 
+    induction R ; intros.
+        - apply bctLJF4_R_box.
+            + destruct p; T_bracketable.
+            + apply eptLJF4_L_False. apply H.
+        - apply bctLJF4_R_box.
+            + T_bracketable. 
+            + apply eptLJF4_L_False. apply H.
+        - apply bctLJF4_R_box.
+            + T_bracketable.
+            + apply eptLJF4_L_False. apply H.
+        - apply bctLJF4_R_box.
+            + T_bracketable.
+            + apply eptLJF4_L_False. apply H.
+        - apply bctLJF4_R_AndN.
+            + apply IHR1. apply H.
+            + apply IHR2. apply H.  
+        - apply bctLJF4_R_box.
+            + T_bracketable.
+            + apply eptLJF4_L_False. apply H.
+        - apply bctLJF4_R_Impl. apply IHR2. apply in_cons. apply H.
+Qed.
+
+Lemma admissibility_L_box : forall (R: o) (C: dctx) (K: o),
+    bctLJF4 C R->
+    forall (C1: dctx),
+      has_entry C (K, omega) ->
+      upd_rel_ex C (K, omega) (K, one) C1 ->
+      bctLJF4 C1 R.
+Admitted.
+
+
