src/rules/LJFPS_Rules.v
@@ -1,0 +1,123 @@
+From Stdlib Require Import List.
+
+From CARVe Require Import contexts.list.
+From CARVe Require Import algebras.structural.
+
+
+From LJF Require Import SharedLogic.
+
+(* structural context -> ordered linear context -> right side formula*)
+Inductive bct : sctx -> octx -> o -> Prop :=
+| bct_R_box :
+  forall {S: sctx} {O: octx} {D: o},
+    bracketable D ->
+    ept S O D->
+    bct S O D
+| bct_R_AndN :
+  forall {S: sctx} {O: octx} {B1 B2: o},
+    bct S O B1 ->
+    bct S O B2 ->
+    bct S O (AndN B1 B2)
+| bct_R_Impl :
+  forall {S : sctx} {O: octx} {B1 B2: o},
+    bct S (B1 :: O) B2 ->
+    bct S O (Impl B1 B2)
+(* structural context -> ordered linear context -> right side formula*)
+with ept : sctx -> octx -> o -> Prop := 
+| ept_L_f :
+  forall {S: sctx} (N: o) {K: o},
+    bracketable K ->
+    has_entry S (N, tt) ->
+    negative N ->
+    lfc S N K ->
+    ept S nil K
+| ept_R_f :
+  forall {S: sctx} {P: o},
+    positive P ->
+    rfc S P ->
+    ept S nil P
+| ept_L_box :
+  forall {S: sctx} {O: octx} {B : o} {K : o},
+    bracketable K ->
+    permeable B ->
+    ept ((B, tt) :: S) O K ->
+    ept S (B :: O) K
+| ept_L_AndP :
+  forall {S: sctx} {O: octx} {B1 B2 : o} {K: o},
+    bracketable K ->
+    ept S (B2 :: (B1 :: O)) K ->
+    ept S ((AndP B1 B2) :: O) K
+| ept_L_Or :
+  forall {S: sctx} {O: octx} {B1 B2 : o}  {K: o},
+    bracketable K ->
+    ept S (B1 :: O) K ->
+    ept S (B2 :: O) K ->
+    ept S ((Or B1 B2) :: O) K
+| ept_L_True :
+  forall {S: sctx} {O: octx}  {K: o},
+    bracketable K ->
+    ept S O K ->
+    ept S (TT :: O) K
+| ept_L_False :
+  forall {S: sctx} {O: octx} {K: o},
+    bracketable K ->
+    ept S (FF :: O) K
+(* structural context -> focused formula -> right side formula*)
+with lfc : sctx -> o -> o -> Prop :=
+| lfc_R_l :
+  forall {S : sctx} {P : o}  {K : o},
+    bracketable K ->
+    positive P ->
+    ept S (P :: nil) K ->
+    lfc S P K
+| lfc_I_l :
+  forall {S: sctx} {N : o},
+    negative N ->
+    atomic N ->
+    lfc S N N
+| lfc_L_AndN_1 :
+  forall {S: sctx} {B1 B2 : o}  {K : o},
+    bracketable K ->
+    lfc S B1 K ->
+    lfc S (AndN B1 B2) K
+| lfc_L_AndN_2 :
+  forall {S: sctx} {B1 B2 : o}  {K : o},
+    bracketable K ->
+    lfc S B2 K ->
+    lfc S (AndN B1 B2) K
+| lfc_L_Impl :
+  forall {S: sctx} {B1 B2 : o}  {K : o},
+    bracketable K ->
+    rfc S B1 ->
+    lfc S B2 K ->
+    lfc S (Impl B1 B2) K
+(* structural context -> focused formula*)
+with rfc : sctx -> o -> Prop :=
+| rfc_R_r :
+  forall {S: sctx} {N: o},
+    negative N ->
+    bct S nil N ->
+    rfc S N
+| rfc_I_r :
+  forall {S: sctx} {P: o},
+    positive P ->
+    atomic P ->
+    has_entry S (P, tt) ->
+    rfc S P
+| rfc_R_AndP :
+  forall {S: sctx} {B1 B2: o},
+    rfc S B1 ->
+    rfc S B2 ->
+    rfc S (AndP B1 B2)
+| rfc_R_Or_1 :
+  forall {S: sctx} {B1 B2: o},
+    rfc S B1 ->
+    rfc S (Or B1 B2)
+| rfc_R_Or_2 :
+  forall {S: sctx} {B1 B2: o},
+    rfc S B2 ->
+    rfc S (Or B1 B2)
+| rfc_R_True :
+  forall {S: sctx}, 
+    rfc S TT
+.
