src/rules/LJF_Rules.v
@@ -1,135 +1,138 @@
 From Stdlib Require Import List.
 
-From CARVe Require Import contexts.list algebras.dill.
+From CARVe Require Import contexts.list.
+From CARVe Require Import algebras.dill.
+
 
 From LJF Require Import SharedLogic.
+
 
 Variant state : Type :=
   | Bracketed : state
   | Unbracketed : state
 .
 
-Inductive ufcLJF : ctx -> o -> state -> Prop :=
+Inductive ufcLJF : dctx -> o -> state -> Prop :=
 | ufcLJF_L_f :
-  forall {C: ctx} {N : o} {K : o},
+  forall {C: dctx} {N : o} {K : o},
     exh C ->
     has_entry C (N, omega) ->
     negative N ->
     lfcLJF C N K ->
     ufcLJF C K Bracketed
 | ufcLJF_R_f :
-  forall {C: ctx} {P: o},
+  forall {C: dctx} {P: o},
     exh C ->
     positive P ->
     rfcLJF C P ->
     ufcLJF C P Bracketed
 | ufcLJF_L_box :
-  forall {C C1 : ctx} {B : o} {K : o} {s : state},
+  forall {C C1 : dctx} {B : o} {K : o} {s : state},
     upd_rel_ex C (B, one) (B, omega) C1 ->
     permeable B ->
     ufcLJF C1 K s ->
     ufcLJF C K s
 | ufcLJF_R_box :
-  forall {C: ctx} {D: o},
+  forall {C: dctx} {D: o},
     bracketable D ->
     ufcLJF C D Bracketed ->
     ufcLJF C D Unbracketed
 | ufcLJF_L_AndP :
-  forall {C C1: ctx} {B1 B2 : o} {K: o} {s : state},
+  forall {C C1: dctx} {B1 B2 : o} {K: o} {s : state},
     has_entry C ((AndP B1 B2), one) ->
     upd_rel_ex C ((AndP B1 B2), one) ((AndP B1 B2), zero) C1 ->
     ufcLJF ((B1, one) :: (B2, one) :: C1) K s ->
     ufcLJF C K s
 | ufcLJF_R_AndN :
-  forall {C: ctx} {B1 B2: o},
+  forall {C: dctx} {B1 B2: o},
     ufcLJF C B1 Unbracketed ->
     ufcLJF C B2 Unbracketed->
     ufcLJF C (AndN B1 B2) Unbracketed
 | ufcLJF_L_Or :
-  forall {C C1: ctx} {B1 B2 : o}  {K: o} {s: state},
+  forall {C C1: dctx} {B1 B2 : o}  {K: o} {s: state},
     has_entry C ((Or B1 B2), one) ->
     upd_rel_ex C ((Or B1 B2), one) ((Or B1 B2), zero) C1 ->
     ufcLJF ((B1, one) :: C1) K s ->
     ufcLJF ((B2, one) :: C1) K s ->
     ufcLJF C K s
 | ufcLJF_R_Impl :
-  forall {C : ctx} {B1 B2: o},
+  forall {C : dctx} {B1 B2: o},
     ufcLJF ((B1, one) :: C) B2 Unbracketed ->
     ufcLJF C (Impl B1 B2) Unbracketed
 | ufcLJF_L_True :
-  forall {C C1: ctx}  {K: o} {s: state},
+  forall {C C1: dctx}  {K: o} {s: state},
     has_entry C (TT, one) ->
     upd_rel_ex C (TT, one) (TT, zero) C1 ->
     ufcLJF C1 K s ->
     ufcLJF C K s
 | ufcLJF_L_False :
-  forall {C: ctx}  {K: o} {s: state},
+  forall {C: dctx}  {K: o} {s: state},
     has_entry C (FF, one) ->
     ufcLJF C K s
 
     (* First o for focused assumption, second o for conclusion K *)
-with lfcLJF : ctx -> o -> o -> Prop :=
+with lfcLJF : dctx -> o -> o -> Prop :=
 | lfcLJF_R_l :
-  forall {C : ctx} {P : o}  {K : o},
+  forall {C : dctx} {P : o}  {K : o},
     exh C ->
     positive P ->
     ufcLJF ((P, one) :: C) K Bracketed ->
     lfcLJF C P K
 | lfcLJF_I_l :
-  forall {C: ctx} {N : o},
+  forall {C: dctx} {N : o},
     exh C ->
     negative N ->
     atomic N ->
     lfcLJF C N N
 | lfcLJF_L_AndN_1 :
-  forall {C: ctx} {B1 B2 : o}  {K : o},
+  forall {C: dctx} {B1 B2 : o}  {K : o},
     exh C ->
     lfcLJF C B1 K ->
     lfcLJF C (AndN B1 B2) K
 | lfcLJF_L_AndN_2 :
-  forall {C: ctx} {B1 B2 : o}  {K : o},
+  forall {C: dctx} {B1 B2 : o}  {K : o},
     exh C ->
     lfcLJF C B2 K ->
     lfcLJF C (AndN B1 B2) K
 | lfcLJF_L_Impl :
-  forall {C: ctx} {B1 B2 : o}  {K : o},
+  forall {C: dctx} {B1 B2 : o}  {K : o},
     exh C ->
     rfcLJF C B1 ->
     lfcLJF C B2 K ->
     lfcLJF C (Impl B1 B2) K
 
-with rfcLJF : ctx -> o -> Prop :=
+with rfcLJF : dctx -> o -> Prop :=
 | rfcLJF_R_r :
-  forall {C: ctx} {N: o},
+  forall {C: dctx} {N: o},
     exh C ->
     negative N ->
     ufcLJF C N Unbracketed ->
     rfcLJF C N
 | rfcLJF_I_r :
-  forall {C: ctx} {P: o},
+  forall {C: dctx} {P: o},
     exh C ->
     has_entry C (P, omega) ->
     positive P ->
     atomic P ->
     rfcLJF C P
 | rfcLJF_R_AndP :
-  forall {C: ctx} {B1 B2: o},
+  forall {C: dctx} {B1 B2: o},
     exh C ->
     rfcLJF C B1 ->
     rfcLJF C B2 ->
     rfcLJF C (AndP B1 B2)
 | rfcLJF_R_Or_1 :
-  forall {C: ctx} {B1 B2: o},
+  forall {C: dctx} {B1 B2: o},
     exh C ->
     rfcLJF C B1 ->
     rfcLJF C (Or B1 B2)
 | rfcLJF_R_Or_2 :
-  forall {C: ctx} {B1 B2: o},
+  forall {C: dctx} {B1 B2: o},
     exh C ->
     rfcLJF C B2 ->
     rfcLJF C (Or B1 B2)
 | rfcLJF_R_True :
-  forall {C: ctx},
+  forall {C: dctx},
     exh C ->
     rfcLJF C TT
 .
